Fiddling

scratch.lean
@@ -2,7 +2,7 @@
 
 
 variables {α β : Type}
-meta def Y : ((α → β) → α → β) → α → β | f x := f (Y f) x
+meta def Y {α : Type} : (α → α) → α | f := f (Y f)
 
 universes u v
 
@@ -16,7 +16,6 @@ def e := Π a : Type u, Π b : Type v, a × b
 #eval to_string $ expr.collect_univ_params $ expr.reflect e
 
 #eval @undefined_core nat "wtf"
-
 
 namespace hidden
 
@@ -40,6 +39,46 @@ do
 
 example : true := begin trace_simp_lemmas, trivial  end
 
+namespace my_namespace
+    constant X : Type u
+    constants x y : X
+    constant f : X → X
+    constants  (P : X → Prop) (Q : Prop)
+    /--Hello world-/
+    axiom my_axiom : ∀ (a:X) (p : P(a)) (q:Q), Q
+    #check my_axiom
+    #check expr.mvar
+    meta def scratch_tac : tactic unit := do
+        -- a ← tactic.resolve_name `my_axiom >>= tactic.to_expr,
+        -- l ← tactic.apply_core a {},
+        -- g ← tactic.target,
+        -- tactic.set_tag g [`hello.world],
+        -- e ← tactic.head_eta_expand a,
+        -- tactic.trace e,
+        tactic.mk_fresh_name >>= tactic.trace,
+        pure()
+
+    example : Q :=
+    begin
+        scratch_tac,
+        scratch_tac,
+        scratch_tac,
+        scratch_tac,
+        tactic.rotate_left 1,
+        sorry
+    end
+    example : true := begin 
+        tactic.add_doc_string `nat "my dumb axiom is great at breaking maths yay.",
+        tactic.doc_string `nat >>= tactic.trace,
+        trivial 
+    end
+    #check nat
+section scratch
+
+end scratch
+end my_namespace
+
+
 end hidden
 
 
@@ -49,3 +88,52 @@ begin
     apply h₂ _, assumption
 end
 
+example : ∀ (n : nat), n = n := 
+begin
+  intro,
+  induction n,
+end
+
+
+namespace field_idea_auto_param
+    -- eventually a sophisticated tactic that figures out if an elt is ≠ 0
+    meta def nz_tactic := tactic.assumption 
+    class dvr (R : Type u) extends (ring R) :=
+    (inv(x:R) (p:x ≠ 0):  R)
+    (inv_l : Π (x y : R) (p:y≠0), x * (inv y p)  = 1 )
+    variables {R : Type u} [dvr R]
+    def inv (y : R) (nz : y ≠ 0 . nz_tactic) : R := dvr.inv y nz
+
+    def div (x y : R) (nz : y ≠ 0 . nz_tactic) : R := x * (inv y)
+    infix ` /. `:50 := div
+
+    variables {x y : R} 
+    variable (xz : x ≠ 0 . nz_tactic) -- I was really hoping that this would be allowed
+
+    example (x y : R) (xz : x ≠ 0) (yz : y ≠ 0) : (1 /. (x * y)) = (1 /. x) * (1 /. y) := sorry
+
+end field_idea_auto_param
+
+namespace field_idea_class
+    class my_division_ring (R : Type u) extends (integral_domain R) :=
+    (inv : Π(x:R) [x ≠ 0],  R)
+    (inv_l (x : R) [nz:x ≠ 0] : x * (@inv x nz)  = 1 )
+    (inv_r (x : R) [nz:x ≠ 0] : (@inv x nz) * x  = 1 )
+
+    variables {R : Type u} [my_division_ring R]
+    def inv (y : R) [nz:y ≠ 0] : R := @my_division_ring.inv _ _ y nz
+
+    def div (x y : R) [y ≠ 0] : R := x * (inv y)
+    infix ` ÷ `:50 := div
+
+    variables {x y : R} [x ≠ 0] [y ≠ 0]
+    def asdf : ((x * y) ≠ 0) := mul_ne_zero ‹x ≠ 0› ‹y ≠ 0›
+
+    example : (1 ÷ (x * y)) = (1 ÷ x) * (1 ÷ y) := sorry
+    -- calc (1 ÷ (x * y)) = inv(x * y) * 1 : by sorry
+    --      ...           = inv(x * y) * (x * inv(x)) * (y * inv(y)) : by sorry
+    --      ...           = (inv(x * y) * (x * y)) * (inv(x) * inv(y)) : by ac_refl
+    --      ...           = 1 * (1 * inv(x)) * (1 * inv(y)) : by sorry
+    --      ...           = (1 ÷ x) * (1 ÷ y) : by sorry
+
+end field_idea_class
