rosser.lean
@@ -1,0 +1,19 @@
+
+universe u
+inductive pred (α : Type u) : Type u
+|and : pred → pred → pred
+|not : pred → pred
+|atom : α → pred
+
+prefix `~` := pred.not
+infixl `&`:50 := pred.and
+def pred.or {α : Type u} : pred α → pred α  → pred α := λ P Q, ~((~P)&(~Q))
+def pred.imp {α : Type u}: pred α  → pred α→ pred α  := λ P Q, ~(P&(~Q))
+infixl `|`:40 := pred.or
+local infixl `⊃`:50 := pred.imp
+instance atom_coe {α} : has_coe (α) (pred α) := ⟨pred.atom⟩
+section
+parameter {α : Type u}
+abbreviation p := pred α
+
+end
